Proved the commutativity theorem using structural relation.

STLC_SuccNat/LR.v
@@ -1,552 +1,122 @@
-From Stdlib Require Import List.
-Import List.ListNotations.
-Open Scope list_scope.
-From STLC Require Import STLC_SuccNat Lifted_STLC_SuccNat Msubst Lifted_Msubst.
+From STLC Require Import Ceval Lifted_Ceval.
 
-(* Fixpoint LR (cfg:feat_config) (T:ty) (t:tm) (t':tm') : Prop :=
-  has_type empty t T /\ has_type' empty t' (lift_ty T) /\
-  match T with
-  | Nat => exists r r',
-	          step_normal_form_of t (const r) /\
-	          step'_normal_form_of t' (const' r') /\
-	          derive r' cfg = Some r
-  | (Arrow T1 T2) => forall arg arg',
-            LR cfg T1 arg arg' ->
-            LR cfg T2 (app t arg) (app' t' arg')
-  end. *)
+Inductive LR (conf:feat_config) : tm -> tm' -> Prop :=
+  | LR_var: forall x, LR conf (var x) (var' x)
+  | LR_app: forall t1 t2 t1' t2',
+    LR conf t1 t1' ->
+    LR conf t2 t2' ->
+    LR conf (app t1 t2) (app' t1' t2')
+  | LR_abs: forall x T t t',
+    LR conf t t' ->
+    LR conf (abs x T t) (abs' x (lift_ty T) t')
+  | LR_fixp: forall t t',
+    LR conf t t' -> LR conf (fixp t) (fixp' t')
+  | LR_const: forall n n',
+    derive n' conf = Some n ->
+    LR conf (const n) (const' n')
+  | LR_succ: forall t t',
+    LR conf t t' ->
+    LR conf (succ t) (succ' t').
 
-Fixpoint LR (cfg:feat_config) (T:ty) (t:tm) (t':tm') : Prop :=
-  has_type empty t T /\ has_type' empty t' (lift_ty T) /\
-  match T with
-  | Nat => exists r r',
-	          step_normal_form_of t (const r) /\
-	          step'_normal_form_of t' (const' r') /\
-	          derive r' cfg = Some r
-  | (Arrow T1 T2) => exists f f',
-            step_normal_form_of t f /\
-            step'_normal_form_of t' f' /\
-            (forall arg arg', LR cfg T1 arg arg' ->
-            LR cfg T2 (app t arg) (app' t' arg'))
-  end.
-
-Lemma LR_typable_empty : forall {cfg} {T} {t} {t'},
-  LR cfg T t t' ->
-  has_type empty t T /\ has_type' empty t' (lift_ty T).
+Lemma subst_LR_subst': forall conf t1 t1' t2 t2' s,
+  LR conf t1 t1' ->
+  LR conf t2 t2' ->
+  LR conf (subst s t2 t1) (subst' s t2' t1').
 Proof.
-  intros.
-  destruct T; unfold LR in H; split;
-    try (destruct H as [H _]; assumption);
-    destruct H as [_ [H _] ]; assumption.
+  intros conf t1 t1' t2 t2' s HLR.
+  induction HLR; intros.
+  - simpl. destruct (eqb_spec s x).
+    assumption. constructor.
+  - simpl. apply LR_app.
+    + apply IHHLR1. assumption.
+    + apply IHHLR2. assumption.
+  - simpl. destruct (eqb_spec s x).
+    + constructor. assumption.
+    + constructor. apply IHHLR. assumption.
+  - simpl. constructor.
+    apply IHHLR. assumption.
+  - simpl. constructor. assumption.
+  - simpl. constructor.
+    apply IHHLR. assumption.
 Qed.
 
-Lemma step_preserves_LR : forall T cfg t1 t2 t', (step t1 t2) -> LR cfg T t1 t' -> LR cfg T t2 t'.
+Lemma cstep_LR_cstep': forall conf t t',
+  LR conf t t' -> LR conf (cstep t) (cstep' t').
 Proof.
- induction T;  intros cfg t1 t2 t' E Rt;
-               destruct Rt as [Hty [Hty' H] ].
-  (* Arrow *)
-  - split; [|split]; auto.
-    eapply preservation; eassumption.
-    clear Hty Hty'.
-    destruct H as [f [f' [Hsnf [Hsnf' H]]]].
-    exists f, f'.
-    apply (st_pr_nf _ _ _ E) in Hsnf.
-    split; [eassumption| split; [eassumption|]].
-    intros.
-    eapply IHT2.
-    eapply ST_App. eassumption.
-    apply H. assumption.
-  (* Nat *)
-  - split; [|split]; auto.
-    eapply preservation; eassumption.
-    destruct H as [r [r' [Hsnf [Hsnf' Hd]]]].
-    exists r, r'. split; [|split]; auto.
-    clear Hsnf' Hd Hty Hty'.
-    destruct Hsnf as [Hms _].
-    split; [|intros [x contra]; inversion contra].
-    inversion Hms; subst;
-      try solve_by_inverts 1.
-    apply (determinism _ _ _ H) in E.
-    rewrite E in *.
+  induction t; intros;
+  inversion H; subst.
+  - constructor.
+  - destruct t1, t1';
+    try solve_by_inverts 1;
+    try (apply IHt1 in H2;
+         constructor; assumption).
+    simpl in *. inversion H2; subst.
+    eapply subst_LR_subst'; assumption.
+  - constructor. assumption.
+  - destruct t, t'0;
+    try solve_by_inverts 1;
+    try (apply IHt in H1;
+         constructor; assumption).
+  - constructor. assumption.
+  - destruct t, t'0;
+    try solve_by_inverts 1;
+    try (apply IHt in H1;
+         constructor; assumption).
+    inversion H1; subst.
+    simpl. constructor.
+    apply mapping_not_change_deriving.
     assumption.
 Qed.
 
-Lemma step'_preserves_LR : forall T cfg t t1' t2', (step' t1' t2') -> LR cfg T t t1' -> LR cfg T t t2'.
+Lemma mcstep_mcstep'__LR: forall conf i t t' v v',
+  LR conf t t' ->
+  mcstep i t = Some v ->
+  mcstep' i t' = Some v' ->
+  LR conf v v'.
 Proof.
- induction T;  intros cfg t t1' t2' E Rt;
-               destruct Rt as [Hty [Hty' H] ].
-  (* Arrow *)
-  - split; [|split]; auto.
-    eapply preservation'; eauto.
-    clear Hty Hty'.
-    destruct H as [f [f' [Hsnf [Hsnf' H]]]].
-    exists f, f'.
-    apply (st_pr_nf' _ _ _ E) in Hsnf'.
-    split; [eassumption| split; [eassumption|]].
-    intros.
-    eapply IHT2.
-    apply ST_App'. eassumption.
-    apply H. assumption.
-  (* Nat *)
-  - split; [|split]; auto.
-    eapply preservation'; eassumption.
-    destruct H as [r [r' [Hsnf [Hsnf' Hd]]]].
-    exists r, r'. split; [|split]; auto.
-    clear Hsnf Hd Hty Hty'.
-    destruct Hsnf' as [Hms' _].
-    split; [|intros [x contra]; inversion contra].
-    inversion Hms'; subst;
-      try solve_by_inverts 1.
-    apply (determinism' _ _ _ H) in E.
-    rewrite E in *.
-    assumption.
+ induction i; intros t t' v v' HLR Hmc Hmc'.
+  - simpl in Hmc, Hmc'.
+    destruct t, t'; subst;
+    try discriminate;
+    try (injection Hmc as Hmc;
+    injection Hmc' as Hmc';
+    subst; assumption).
+  - eapply IHi.
+    + eapply cstep_LR_cstep' in HLR.
+      exact HLR.
+    + pose proof (mcstep_Si i t v) as [H _].
+      apply H. assumption.
+    + pose proof (mcstep'_Si i t' v')as [H _].
+      apply H. exact Hmc'.
 Qed.
 
-Lemma step_preserves_LR' : forall T cfg t1 t2 t',
-  has_type empty t1 T -> 
-  (step t1 t2) ->
-  LR cfg T t2 t' -> LR cfg T t1 t'.
+Lemma derive_LR: forall conf n' n,
+  derive n' conf = Some n ->
+  LR conf (const n) (const' n').
 Proof.
- induction T;  intros cfg t1 t2 t' HT E Rt;
-               destruct Rt as [Hty [Hty' H] ].
-  (* Arrow *)
-  - split; [|split]; auto.
-    destruct H as [f [f' [Hsnf [Hsnf' H]]]].
-    exists f, f'.
-    apply (st_exp_pr_nf _ _ _ E) in Hsnf.
-    split; [eassumption| split;[eassumption|]].
-    intros.
-    eapply IHT2.
-    eapply T_App. eauto.
-    eapply LR_typable_empty; eauto.
-    apply ST_App. apply E.
-    apply H. assumption.
-  (* Nat *)
-  - split; [|split]; auto.
-    destruct H as [r [r' [Hsnf [Hsnf' Hd]]]].
-    exists r, r'. split; [|split]; auto.
-    clear Hsnf' Hd Hty Hty'.
-    destruct Hsnf as [Hms _].
-    split; [|intros [x contra]; inversion contra].
-    eapply multi_step; eassumption.
+  intros. constructor. assumption.
 Qed.
 
-Lemma step'_preserves_LR' : forall T cfg t t1' t2',
-  has_type' empty t1' (lift_ty T) -> 
-  (step' t1' t2') ->
-  LR cfg T t t2' -> LR cfg T t t1'.
+Lemma lift_LR: forall conf t,
+  LR conf t (lift t).
 Proof.
- induction T;  intros cfg t t1' t2' HT E Rt;
-               destruct Rt as [Hty [Hty' H] ].
-  (* Arrow *)
-  - split; [|split]; auto.
-    clear Hty'.
-    destruct H as [f [f' [Hsnf [Hsnf' H]]]].
-    exists f, f'.
-    apply (st_exp_pr_nf' _ _ _ E) in Hsnf'.
-    split; [eassumption| split; [eassumption|]].
-    intros.
-    eapply IHT2.
-    eapply T_App'. eauto.
-    eapply LR_typable_empty; eauto.
-    apply ST_App'. apply E.
-    apply H. assumption.
-  (* Nat *)
-  - split; [|split]; auto.
-    destruct H as [r [r' [Hsnf [Hsnf' Hd]]]].
-    exists r, r'. split; [|split]; auto.
-    clear Hsnf Hd Hty Hty'.
-    destruct Hsnf' as [Hms' _].
-    split; [|intros [x contra]; inversion contra].
-    eapply multi_step; eassumption.
+  induction t;
+  try (constructor; assumption).
+  - constructor. reflexivity.
 Qed.
-
-Lemma mstep_preserves_LR': forall T cfg t1 t2 t',
-  has_type empty t1 T ->
-  multi step t1 t2 ->
-  LR cfg T t2 t' -> LR cfg T t1 t'.
+ 
+Theorem commutativity: forall conf i analysis spl p r r',
+  derive spl conf = Some p ->
+  mcstep i (app analysis (const p)) = Some (const r) ->
+  mcstep' i (app' (lift analysis) (const' spl)) = Some (const' r') ->
+  derive r' conf = Some r.
 Proof.
-  intros. induction H0.
-  - assumption.
-  - apply (preservation _ _ _ H) in H0 as H3.
-    apply (IHmulti H3) in H1.
-    eapply step_preserves_LR'; eauto.
-Qed.
-
-Lemma mstep_preserves_LR: forall T cfg t1 t2 t',
-  multi step t1 t2 ->
-  LR cfg T t1 t' -> LR cfg T t2 t'.
-Proof.
-  intros. induction H.
-  - assumption.
-  - apply IHmulti.
-    eapply step_preserves_LR; eauto.
-Qed.
-
-Lemma mstep'_preserves_LR': forall T cfg t t1' t2',
-  has_type' empty t1' (lift_ty T) ->
-  multi step' t1' t2' ->
-  LR cfg T t t2' -> LR cfg T t t1'.
-Proof.
-  intros. induction H0.
-  - assumption.
-  - apply (preservation' _ _ _ H) in H0 as H3.
-    apply (IHmulti H3) in H1.
-    eapply step'_preserves_LR'; eauto.
-Qed.
-
-Lemma mstep'_preserves_LR: forall T cfg t t1' t2',
-  multi step' t1' t2' ->
-  LR cfg T t t1' -> LR cfg T t t2'.
-Proof.
-  intros. induction H.
-  - assumption.
-  - apply IHmulti.
-    eapply step'_preserves_LR; eauto.
-Qed.
-
-Lemma mstep_mstep'__preserves_LR: forall T cfg t1 t2 t1' t2',
-  multi step t1 t2 ->
-  multi step' t1' t2' ->
-  LR cfg T t1 t1' -> LR cfg T t2 t2'.
-Proof.
-  intros.
-  apply (mstep'_preserves_LR _ _ _ _ t2') in H1; auto.
-  apply (mstep_preserves_LR _ _ _ t2) in H1; auto.
-Qed.
-
-Lemma mstep_mstep'__preserves_LR': forall T cfg t1 t2 t1' t2',
-  has_type empty t1 T ->
-  has_type' empty t1' (lift_ty T) ->
-  multi step t1 t2 ->
-  multi step' t1' t2' ->
-  LR cfg T t2 t2' -> LR cfg T t1 t1'.
-Proof.
-  intros.
-  apply (preservation'_multi _ _ _ H0) in H2 as H4.
-  apply (mstep'_preserves_LR' _ _ _ t1') in H3; auto.
-  apply (preservation_multi _ _ _ H) in H1 as H5.
-  apply (mstep_preserves_LR' _ _ t1) in H3; auto.
-Qed.  
-  
-Lemma soundness: forall cfg analysis,
-  LR cfg (Arrow Nat Nat) analysis (lift analysis) ->
-  (forall spl p r' r,
-    derive spl cfg = Some p ->
-    step_normal_form_of (app analysis (const p)) (const r) ->
-    step'_normal_form_of (app' (lift analysis) (const' spl)) (const' r') ->
-    derive r' cfg = Some r
-  ).
-Proof.
-  intros cfg analysis HLR spl p r' r Hd Hsnf Hsnf'.
-  unfold LR in HLR. destruct HLR as [HT [HT' [f [f' [_ [_ HLR]]]]]].
-  specialize HLR with (arg:=(const p)) (arg':=(const' spl)).
-  destruct HLR.
-  { split; [|split]; auto.
-    exists p, spl; split; [|split];
-      try (split;[apply multi_refl| intros [x contra]; inversion contra]);
-      assumption. }
-  destruct H0 as [_ [r0 [r0' [Hsnf0 [Hsnf0' Hd0']]]]].
-
-  apply (normal_forms_unique _ _ _ Hsnf0) in Hsnf.
-  injection Hsnf as Hsnf; subst.
-
-  apply (normal_forms'_unique _ _ _ Hsnf0') in Hsnf'.
-  injection Hsnf' as Hsnf'; subst.
-
+  intros conf i analysis spl p r r' Hd Hmc Hmc'.
+  pose proof (derive_LR conf spl p Hd).
+  pose proof (lift_LR conf analysis).
+  pose proof (LR_app _ _ _ _ _ H0 H).
+  pose proof (mcstep_mcstep'__LR _ _ _ _ _ _ H1 Hmc Hmc').
+  clear - H2.
+  inversion H2; subst.
   assumption.
-Qed.
-
-Require Import Environments.
-
-Inductive instantiation : feat_config -> tass -> env -> env' -> Prop :=
-  | V_nil : forall cfg, instantiation cfg nil nil nil
-  | V_cons : forall cfg x T t t' c e e',
-    instantiation cfg c e e'->
-    LR cfg T t t' ->
-    instantiation cfg ((x,T)::c) ((x,t)::e) ((x,t')::e').
-
-Lemma instantiation_domains_match: forall {cfg} {c} {e} {e'},
-  instantiation cfg c e e'->
-  forall {x} {T},
-    lookup x c = Some T -> 
-      exists t, lookup x e = Some t /\ 
-      exists t', lookup x e' = Some t'.
-Proof.
-  intros cfg x e e' V. induction V; intros x0 T0 C.
-    solve_by_inverts 1.
-    simpl in *.
-    destruct (eqb x x0); eauto.
-Qed.
-
-Lemma instantiation_LR : forall cfg c e e',
-  instantiation cfg c e e' ->
-  forall x t t' T,
-    lookup x c = Some T ->
-    lookup x e = Some t ->
-    lookup x e' = Some t' ->
-    LR cfg T t t'.
-Proof.
-  intros cfg c e e' V.
-  induction V; intros x0 t1 t1' T0 Hc He He'.
-  - solve_by_inverts 1.
-  - simpl in Hc, He, He'.
-    destruct (eqb x x0).
-    + injection Hc as HT.
-      injection He as Hv.
-      injection He' as Hv'.
-      subst. assumption.
-    + eauto.
-Qed.
-
-Lemma instantiation_env_closed: forall cfg c e e',
-  instantiation cfg c e e' -> closed_env e /\ closed'_env' e'.
-Proof.
-  intros cfg c e e' Hinst.
-  induction Hinst.
-  - split; constructor.
-  - destruct IHHinst as [He He'].
-    split.
-    + unfold closed_env; fold closed_env.
-      split; [|assumption].
-      eapply typable_empty__closed.
-      eapply LR_typable_empty.
-      eassumption.
-    + unfold closed'_env'; fold closed'_env'.
-      split; [|assumption].
-      eapply typable_empty__closed'.
-      eapply LR_typable_empty.
-      eassumption.
-Qed.
-
-Lemma msubst_preserves_typing : forall cfg c e e',
-  instantiation cfg c e e' ->
-  forall Gamma t S, has_type (mupdate Gamma c) t S ->
-  has_type Gamma (msubst e t) S.
-Proof.
-    intros cfg c e e' H. induction H; intros.
-    simpl in H. simpl. auto.
-    simpl in H1.  simpl.
-    apply IHinstantiation.
-    eapply substitution_preserves_typing; eauto.
-    apply (LR_typable_empty H0).
-Qed.
-
-Fixpoint lift_tass (c:tass) : tass' :=
-  match c with
-  | nil => nil
-  | (x,T)::ts => (x,(lift_ty T)) :: (lift_tass ts)
-  end.
-
-Lemma lift_tass_drop: forall x c, lift_tass (drop x c) = drop x (lift_tass c).
-Proof.
-  intros. induction c; auto.
-  simpl. destruct a. simpl.
-  destruct (eqb_spec s x).
-  assumption.
-  simpl. f_equal. assumption.
-Qed.
-
-Lemma msubst'_preserves_typing : forall cfg c e e',
-  instantiation cfg c e e' ->
-  forall Gamma' t' S', has_type' (mupdate' Gamma' (lift_tass c)) t' S' ->
-  has_type' Gamma' (msubst' e' t') S'.
-Proof.
-    intros cfg c e e' H. induction H; intros.
-    simpl in H. simpl. auto.
-    simpl in H0. simpl.
-    apply IHinstantiation.
-    simpl in H1.
-    eapply substitution_preserves_typing'; eauto.
-    apply (LR_typable_empty H0).
-Qed.
-
-Lemma instantiation_drop : forall cfg c env env',
-    instantiation cfg c env env' ->
-    forall x, instantiation cfg (drop x c) (drop x env) (drop x env').
-Proof.
-  intros cfg c e e' V. induction V.
-    intros.  simpl.  constructor.
-    intros. unfold drop.
-    destruct (String.eqb x x0); auto. constructor; eauto.
-Qed.
-
-Lemma completeness: forall c env env' t T cfg,
-  has_type (mupdate empty c)  t T ->
-  instantiation cfg c env env' ->
-  LR cfg T (msubst env t) (msubst' env' (lift t)).
-Proof.
-  intros c env0 env0' t T cfg HT V.
-  generalize dependent env0'.
-  generalize dependent env0.
-  remember (mupdate empty c) as Gamma.
-  assert (forall x, Gamma x = lookup x c).
-    intros. rewrite HeqGamma. rewrite mupdate_lookup. reflexivity.
-  clear HeqGamma.
-  generalize dependent c.
-  induction HT; simpl; intros.
-  - (* T_Var *)
-    rewrite H0 in H.
-    destruct (instantiation_domains_match V H) as [t [P [t' P'] ] ].
-    eapply instantiation_LR; eauto.
-    * rewrite msubst_var.
-      rewrite P; reflexivity.
-      eapply instantiation_env_closed; eauto.
-    * rewrite msubst'_var'.
-      rewrite P'; reflexivity.
-      eapply instantiation_env_closed; eauto.
-  - (* T_Abs *)
-    rewrite msubst_abs, msubst'_abs'.
-    assert (Hty: has_type empty (abs x T2 (msubst (drop x env0) t)) (Arrow T2 T1)).
-    { apply T_Abs. eapply msubst_preserves_typing.
-      apply instantiation_drop; eauto.
-      eapply context_invariance. apply HT.
-      intros.
-      unfold update, t_update. rewrite mupdate_drop. destruct (eqb_spec x x0).
-      + auto.
-      + rewrite H.
-        clear - c n. induction c.
-        simpl. rewrite false_eqb_string; auto.
-        simpl. destruct a.  unfold update, t_update.
-        destruct (String.eqb s x0); auto. }
-     assert (Hty': has_type' empty (abs' x (lift_ty T2) (msubst' (drop x env0') (lift t)))
-              (Arrow' (lift_ty T2) (lift_ty T1))).
-     { apply T_Abs'. eapply msubst'_preserves_typing.
-      apply instantiation_drop; eauto.
-      eapply context'_invariance.
-      apply lifting_types in HT. apply HT.
-      intros.
-      unfold lift_context.
-      unfold update, t_update.
-      rewrite lift_tass_drop, mupdate'_drop.
-      destruct (eqb_spec x x0).
-      + auto.
-      + rewrite H.
-        clear - c n. induction c.
-        simpl. rewrite false_eqb_string; auto.
-        simpl. destruct a. simpl.
-        unfold update, t_update.
-        destruct (String.eqb s x0); auto. }
-     split; [|split]; auto.
-     exists (abs x T2 (msubst (drop x env0) t)),
-            (abs' x (lift_ty T2) (msubst' (drop x env0') (lift t))).
-     repeat split;
-      try apply multi_refl;
-      try (intros [x0 contra]; inversion contra).
-     intros. specialize IHHT with (c:=((x,T2)::c)).
-     assert (forall x0 : string, (x) |-> T2; Gamma x0 = lookup x0 ((x, T2) :: c)).
-     { intros. unfold update, t_update, lookup. destruct (String.eqb x x0); auto. }
-     eapply IHHT in H1.
-     apply mstep_mstep'__preserves_LR' with (msubst ((x,arg)::env0) t) (msubst' ((x,arg')::env0') (lift t)).
-      { eapply T_App; eauto.
-        eapply LR_typable_empty; eauto. }
-      { eapply T_App'; eauto.
-        eapply LR_typable_empty; eauto. }
-      { eapply multi_step. apply ST_AppAbs.
-        simpl. rewrite subst_msubst. apply multi_refl.
-          eapply typable_empty__closed.
-            apply (LR_typable_empty H0).
-            eapply instantiation_env_closed; eauto. }
-      { eapply multi_step. apply ST_AppAbs'.
-        simpl. rewrite subst'_msubst'. apply multi_refl.
-        eapply typable_empty__closed'.
-        apply (LR_typable_empty H0).
-        eapply instantiation_env_closed; eauto.  }
-        eassumption.
-        constructor; auto.
-  - (* T_App *)
-    rewrite msubst_app, msubst'_app'.
-    pose proof (IHHT1 c H env0 env0' V).
-    unfold LR in H0; fold LR in H0.
-    destruct H0 as [HT [HT' [f [f' [_ [_ HLR]]]]]].
-    pose proof (IHHT2 c H env0 env0' V).
-    auto.
-  - (* T_Fixp *)
-    rewrite msubst_fixp, msubst'_fixp'.
-    pose proof (IHHT c H env0 env0' V).
-    pose proof (IHHT c H env0 env0' V).
-    unfold LR in H0; fold LR in H0.
-    destruct H0 as [HT1 [HT1' [f [f' [Hf [Hf' HLR]]]]]].
-    clear IHHT.
-    eapply mstep_mstep'__preserves_LR' with (fixp f) (fixp' f');
-      try eauto.
-    eapply multistep_fixp. apply Hf.
-    eapply multistep'_fixp'. apply Hf'.
-    destruct Hf. 
-    pose proof (preservation_multi _ f _ HT1 H0).
-    pose proof (wt_nf__value _ _ f HT1) as [H4 _].
-    destruct H4 as [_ H4].
-      split; assumption.
-    pose proof (canonical_forms_fun f T1 T1 H3 H4)
-      as [x0 [u H5]]. subst. clear H4 H3 H2.
-    destruct Hf'. 
-    pose proof (preservation'_multi _ f' _ HT1' H2).
-    pose proof (wt_nf__value' _ _ f' HT1') as [H5 _].
-    destruct H5 as [_ H5].
-      split; assumption.
-    pose proof (canonical_forms_fun' f' (lift_ty T1) (lift_ty T1) H4 H5)
-      as [x0' [u' H6]]. subst. clear H5 H4 H3.
-    apply (mstep_mstep'__preserves_LR _ _ _ _ _ _ H0 H2) in H1.
-    assert (forall arg arg', LR cfg T1 arg arg' ->
-              LR cfg T1 (app (abs x0 T1 u) arg)
-                        (app' (abs' x0' (lift_ty T1) u') arg')).
-    { intros.
-      eapply mstep_mstep'__preserves_LR.
-      eapply multistep_app. eassumption.
-      eapply multistep'_app'. eassumption.
-      apply HLR. assumption. }
-    clear HLR.
-    eapply LR_typable_empty in H1 as [HT2 HT2'].
-    eapply mstep_mstep'__preserves_LR'.
-    constructor; assumption.
-    constructor; assumption.
-    eapply multi_step. apply ST_FixpAbs. apply multi_refl.
-    eapply multi_step. apply ST_FixpAbs'. apply multi_refl.
-    apply H3.
-    - (* T_Const *)
-    split; [|split].
-    rewrite msubst_const. auto.
-    rewrite msubst'_const'. auto.
-    exists n, [(n,pc_True)].
-    split; [|split].
-    + rewrite msubst_const. split;
-        [eapply multi_refl
-        | intros [x contra]; inversion contra].
-    + rewrite msubst'_const'. split;
-        [eapply multi_refl
-        | intros [x contra]; inversion contra].
-    + reflexivity.
-  - (* T_Succ *)
-    destruct (IHHT c H env0 env0' V) as [HT0 [HT' [r [r' [ [Hms _] [ [Hms' _] Hd] ] ] ] ] ].
-    split; [|split].
-    rewrite msubst_succ. auto.
-    rewrite msubst'_succ'. auto.
-    eexists; eexists.
-    split; [|split].
-    + rewrite msubst_succ. split;
-        [|intros [x contra]; inversion contra].
-        eapply multi_step_trans.
-        apply multistep_succ; eassumption.
-        eauto.
-    + rewrite msubst'_succ'. split;
-        [|intros [x contra]; inversion contra].
-        eapply multi_step'_trans.
-        apply multistep'_succ'; eassumption.
-        eauto.
-    + apply mapping_not_change_deriving. assumption.
-Admitted.
-
-Theorem commutativity: forall cfg analysis spl p r r',
-  has_type empty analysis (Arrow Nat Nat) ->
-  derive spl cfg = Some p ->
-  (* ceval n (app analysis (const p)) (const r) *)
-  step_normal_form_of (app analysis (const p)) (const r) ->
-  step'_normal_form_of (app' (lift analysis) (const' spl)) (const' r') ->
-  derive r' cfg = Some r.
-Proof.
-  intros cfg analysis spl p r r' HLR.
-  apply soundness.
-  replace (lift analysis) with (msubst' nil (lift analysis)) by reflexivity.
-  replace analysis with (msubst nil analysis) by reflexivity.
-  apply (completeness nil); auto.
-  apply V_nil.
 Qed.
